finish updating Defs

parser/Defs.v
@@ -87,7 +87,7 @@ Module DefsFn (Export Ty : SYMBOL_TYPES).
   Module Export NP  := FSetProperties.Properties NtSet.
   Module Export NE  := FSetEqProperties.EqProperties NtSet.
   Module Export ND  := FSetDecide.Decide NtSet.
-  (* Hide an alternative definition of "sum" from NtSet *)
+  (* hide an alternative definition of "sum" from NtSet *)
   Definition sum := Datatypes.sum.
 
   Definition fromNtList (ls : list nonterminal) : NtSet.t :=
@@ -98,12 +98,12 @@ Module DefsFn (Export Ty : SYMBOL_TYPES).
            (l : list nonterminal), 
       In x l <-> NtSet.In x (fromNtList l).
   Proof.
-    intros x l; split; intro hi; induction l as [| x' l IH]; sis; try ND.fsetdec.
+    intros x l; split; intro hi; induction l as [| x' l Ih]; sis; try ND.fsetdec.
     - destruct hi as [hh | ht]; subst; auto.
       + ND.fsetdec.
-      + apply IH in ht; ND.fsetdec.
+      + apply Ih in ht; ND.fsetdec.
     - destruct (NF.eq_dec x' x); subst; auto.
-      right; apply IH; ND.fsetdec.
+      right; apply Ih; ND.fsetdec.
   Qed.
 
   (* Grammar symbols *)
@@ -227,7 +227,7 @@ Module DefsFn (Export Ty : SYMBOL_TYPES).
   Qed.
 
   (* The semantic type for a list of symbols *)
-  Definition rhs_semty (gamma : list symbol) : Type :=
+  Definition symbols_semty (gamma : list symbol) : Type :=
     tuple (List.map symbol_semty gamma).
 
   (* Grammar productions *)
@@ -242,11 +242,11 @@ Module DefsFn (Export Ty : SYMBOL_TYPES).
 
   (* The type of a semantic predicate for a production *)
   Definition predicate_semty (p : production) : Type :=
-    let (_, ys) := p in rhs_semty ys -> bool.
+    let (_, ys) := p in symbols_semty ys -> bool.
   
   (* The type of a semantic action for a production *)
   Definition action_semty (p : production) : Type :=
-    let (x, ys) := p in rhs_semty ys -> nt_semty x.
+    let (x, ys) := p in symbols_semty ys -> nt_semty x.
 
   Module Production_as_UOT <: UsualOrderedType := Pair_as_UOT NT_as_UOT Gamma_as_UOT.
 
@@ -254,6 +254,17 @@ Module DefsFn (Export Ty : SYMBOL_TYPES).
   Module PM  := FMapAVL.Make Production_as_UOT.
   Module PMF := FMapFacts.Facts PM.
 
+  Lemma grammar_eq_key_elt_equivalence :
+    forall (A : Type),
+      Equivalence (PM.eq_key_elt (elt:=A)).
+  Proof.
+    constructor; try firstorder.
+    - intros x y z heq heq'.
+      repeat red in heq; repeat red in heq'; repeat red.
+      destruct heq as [h1 h2]; destruct heq' as [h3 h4].
+      rewrite h1; rewrite h3; rewrite h2; rewrite h4; auto.
+  Qed.
+  
   (* Grammars *)
 
   (* Each grammar production includes an optional semantic 
@@ -299,13 +310,13 @@ Module DefsFn (Export Ty : SYMBOL_TYPES).
     forall (g    : grammar)
            (p p' : production)
            (fs   : production_semty p')
-           (Hw   : grammar_wf g)
-           (Hf   : PM.find p g = Some (@existT _ _ p' fs)),
+           (hw   : grammar_wf g)
+           (hf   : PM.find p g = Some (@existT _ _ p' fs)),
       production_semty p.
   Proof.
-    intros g p p' fs Hw Hf.
-    apply PMF.find_mapsto_iff in Hf.
-    apply Hw in Hf; subst; auto.
+    intros g p p' fs hw hf.
+    apply PMF.find_mapsto_iff in hf.
+    apply hw in hf; subst; auto.
   Defined.
 
   Lemma in_find_contra :
@@ -314,7 +325,7 @@ Module DefsFn (Export Ty : SYMBOL_TYPES).
       PM.In p g
       -> PM.find p g <> None.
   Proof.
-    intros p g Hi Hf.
+    intros p g hi hf.
     eapply PMF.in_find_iff; eauto.
   Defined.
 
@@ -323,15 +334,15 @@ Module DefsFn (Export Ty : SYMBOL_TYPES).
   Definition findPredicateAndAction
              (p  : production)
              (g  : grammar)
-             (Hw : grammar_wf g)
-             (Hi : PM.In p g) : production_semty p :=
+             (hw : grammar_wf g)
+             (hi : PM.In p g) : production_semty p :=
     match PM.find p g as o return PM.find p g = o -> _ with
     | Some (@existT _ _ _ fs) =>
-      fun Hf =>
-        (coerce_production_semty _ _ _ fs Hw Hf)
+      fun hf =>
+        (coerce_production_semty _ _ _ fs hw hf)
     | None =>
-      fun Hf =>
-        match in_find_contra _ _ Hi Hf with end
+      fun hf =>
+        match in_find_contra _ _ hi hf with end
     end eq_refl.
 
   (* An rhs_map maps each grammar nonterminal to its
@@ -350,13 +361,16 @@ Module DefsFn (Export Ty : SYMBOL_TYPES).
            (m : NM.t A),
       NM.find x m = Some a -> NM.In x m.
   Proof.
-    intros x A a m Hi.
+    intros x A a m hi.
     apply NMF.in_find_iff; tc.
   Qed.
 
   Definition rhs_map := NM.t (list (list symbol)).
 
-  Definition addProduction (p : production) (e : grammar_entry) (rm : rhs_map) : rhs_map :=
+  Definition addProduction
+             (p : production)
+             (e : grammar_entry)
+             (rm : rhs_map) : rhs_map :=
     match p with
     | (x, ys) =>
       match NM.find x rm with
@@ -423,16 +437,6 @@ Module DefsFn (Export Ty : SYMBOL_TYPES).
     - apply rmks'_empty.
     - apply addProduction_preserves_rmks'.
   Qed.
-  
-  Lemma grammar_eq_key_elt_equivalence :
-    Equivalence (PM.eq_key_elt (elt:=grammar_entry)).
-  Proof.
-    constructor; try firstorder.
-    - intros x y z heq heq'.
-      repeat red in heq; repeat red in heq'; repeat red.
-      destruct heq as [h1 h2]; destruct heq' as [h3 h4].
-      rewrite h1; rewrite h3; rewrite h2; rewrite h4; auto.
-  Qed.
 
   Definition rhs_map_keys_sound (rm : rhs_map) (g : grammar) : Prop :=
     forall x,
@@ -463,7 +467,7 @@ Module DefsFn (Export Ty : SYMBOL_TYPES).
   Lemma rms'_empty :
       rms' (NM.empty (list (list symbol))) [].
   Proof.
-    intros x ys yss Hm Hi.
+    intros x ys yss hm hi.
     exfalso.
     eapply NMF.empty_mapsto_iff; eauto.
   Qed.
@@ -473,35 +477,35 @@ Module DefsFn (Export Ty : SYMBOL_TYPES).
       rms' rm prs
       -> rms' (addProduction (fst pr) (snd pr) rm) (prs ++ [pr]).
   Proof.
-    intros rm ((x', ys'), e) prs Hr x ys yss Hm Hi; sis. 
-    destruct (NM.find _ _) as [yss' |] eqn:Hf.
-    - destruct (nt_eq_dec x' x) as [? | Hneq]; subst.
-      + apply NMF.add_mapsto_iff in Hm.
-        destruct Hm as [[_ Heq] | [? ?]]; tc; subst.
-        destruct Hi as [Hh | Ht]; subst.
+    intros rm ((x', ys'), e) prs hr x ys yss hm hi; sis. 
+    destruct (NM.find _ _) as [yss' |] eqn:hf.
+    - destruct (nt_eq_dec x' x) as [? | hneq]; subst.
+      + apply NMF.add_mapsto_iff in hm.
+        destruct hm as [[_ heq] | [? ?]]; tc; subst.
+        destruct hi as [hh | ht]; subst.
         * exists e.
           apply in_or_app; right.
           apply in_eq.
-        * apply NMF.find_mapsto_iff in Hf.
-          eapply Hr in Ht; eauto.
-          destruct Ht as [e' Hi].
+        * apply NMF.find_mapsto_iff in hf.
+          eapply hr in ht; eauto.
+          destruct ht as [e' hi].
           exists e'.
           apply in_or_app; left; auto.
-      + apply NM.add_3 in Hm; auto.
-        eapply Hr in Hi; eauto.
-        destruct Hi as [e' Hi].
+      + apply NM.add_3 in hm; auto.
+        eapply hr in hi; eauto.
+        destruct hi as [e' hi].
         exists e'.
         apply in_or_app; left; auto.
-    - destruct (nt_eq_dec x' x) as [? | Hneq]; subst.
-      + apply NMF.add_mapsto_iff in Hm.
-        destruct Hm as [[_ Heq] | [? ?]]; tc; subst.
-        apply in_singleton_eq in Hi; subst.
+    - destruct (nt_eq_dec x' x) as [? | hneq]; subst.
+      + apply NMF.add_mapsto_iff in hm.
+        destruct hm as [[_ heq] | [? ?]]; tc; subst.
+        apply in_singleton_eq in hi; subst.
         exists e.
         apply in_or_app; right.
         apply in_eq.
-      + apply NM.add_3 in Hm; auto.
-        eapply Hr in Hi; eauto.
-        destruct Hi as [e' Hi].
+      + apply NM.add_3 in hm; auto.
+        eapply hr in hi; eauto.
+        destruct hi as [e' hi].
         exists e'.
         apply in_or_app; left; auto.
   Qed.
@@ -528,11 +532,11 @@ Module DefsFn (Export Ty : SYMBOL_TYPES).
     forall g,
       rhs_map_sound (mkRhsMap g) g.
   Proof.
-    intros g x ys yss Hm Hi.
-    unfold mkRhsMap in Hm.
-    rewrite PM.fold_1 in Hm.
-    eapply rms'__fold_left in Hi; eauto.
-    destruct Hi as [e Hi].
+    intros g x ys yss hm hi.
+    unfold mkRhsMap in hm.
+    rewrite PM.fold_1 in hm.
+    eapply rms'__fold_left in hi; eauto.
+    destruct hi as [e hi].
     apply PMF.elements_in_iff.
     exists e.
     apply In_InA; auto.
@@ -549,8 +553,8 @@ Module DefsFn (Export Ty : SYMBOL_TYPES).
   Lemma rmc'_empty :
       rmc' (NM.empty (list (list symbol))) [].
   Proof.
-    intros x ys e Hi.
-    inv Hi. 
+    intros x ys e hi.
+    inv hi. 
   Qed.
 
   Lemma addProduction_preserves_rmc' :
@@ -605,7 +609,7 @@ Module DefsFn (Export Ty : SYMBOL_TYPES).
       InA (PM.eq_key_elt (elt:=grammar_entry)) ((x, ys), e) prs
       -> In ((x, ys), e) prs.
   Proof.
-    intros x ys e prs hi; induction prs as [| ((x', ys'), e') prs IH]; sis.
+    intros x ys e prs hi; induction prs as [| ((x', ys'), e') prs Ih]; sis.
     - inv hi.
     - inversion hi as [pr' prs' heq | pr' prs' hi']; subst; clear hi.
       + repeat red in heq; sis.
@@ -629,10 +633,24 @@ Module DefsFn (Export Ty : SYMBOL_TYPES).
     rewrite PM.fold_1; auto.
   Qed.
 
+  (* Correctness spec for mkRhsMap *)
   Definition rhs_map_correct (rm : rhs_map) (g : grammar) :=
     rhs_map_keys_sound rm g
     /\ rhs_map_sound rm g
     /\ rhs_map_complete rm g.
+
+  Lemma in_grammar_find_some :
+    forall g rm x ys,
+      rhs_map_correct rm g
+      -> PM.In (x, ys) g
+      -> exists yss,
+          NM.find x rm = Some yss
+          /\ In ys yss.
+  Proof.
+    intros g rm x ys [hs [hs' hc]] hi.
+    apply hc in hi; destruct hi as [yss [hm hi]].
+    apply NMF.find_mapsto_iff in hm; eauto.
+  Qed.
   
   Lemma mkRhsMap_correct :
     forall (g : grammar),
@@ -644,40 +662,24 @@ Module DefsFn (Export Ty : SYMBOL_TYPES).
     - apply mkRhsMap_complete.
   Qed.
 
+  Definition keys (rm : rhs_map) : list nonterminal :=
+    fold_right (fun pr l => fst pr :: l) [] (NM.elements rm).
 
+  Definition keySet (rm : rhs_map) : NtSet.t :=
+    fromNtList (keys rm).
   
-
-  Lemma in_grammar_find_some :
-    forall g pm x ys,
-      production_map_correct pm g
-      -> In (x, ys) g
-      -> exists yss,
-          NM.find x pm = Some yss
-          /\ In ys yss.
-  Proof.
-    intros g pm x ys [hs [hs' hc]] hi.
-    apply hc in hi; destruct hi as [yss [hm hi]].
-    apply NMF.find_mapsto_iff in hm; eauto.
-  Qed.
-
-  Definition keys (pm : production_map) : list nonterminal :=
-    fold_right (fun pr l => fst pr :: l) [] (NM.elements pm).
-
-  Definition keySet (pm : production_map) : NtSet.t :=
-    fromNtList (keys pm).
-  
-  Definition rhssFor (x : nonterminal) (pm : production_map) : list (list symbol) :=
-    match NM.find x pm with
+  Definition rhssFor (x : nonterminal) (rm : rhs_map) : list (list symbol) :=
+    match NM.find x rm with
     | Some yss => yss
     | None     => []
     end.
   
   Lemma rhssFor_in_iff :
-    forall g pm x ys,
-      production_map_correct pm g
-      -> In ys (rhssFor x pm) <-> In (x, ys) g.
+    forall g rm x ys,
+      rhs_map_correct rm g
+      -> In ys (rhssFor x rm) <-> PM.In (x, ys) g.
   Proof.
-    unfold rhssFor; intros g pm x ys [hs [hs' hc]]; split; intros hi.
+    unfold rhssFor; intros g rm x ys [hs [hs' hc]]; split; intros hi.
     - destruct (NM.find _ _) eqn:hf; try inv hi.
       apply NMF.find_mapsto_iff in hf; eauto.
     - apply hc in hi; destruct hi as [yss [hm hi]].
@@ -687,10 +689,10 @@ Module DefsFn (Export Ty : SYMBOL_TYPES).
   Qed.
 
   Lemma rhssFor_keySet :
-    forall x ys pm,
-      In ys (rhssFor x pm) -> NtSet.In x (keySet pm).
+    forall x ys rm,
+      In ys (rhssFor x rm) -> NtSet.In x (keySet rm).
   Proof.
-    intros x ys pm hi; unfold rhssFor in hi.
+    intros x ys rm hi; unfold rhssFor in hi.
     destruct (NM.find _ _) as [yss |] eqn:hf; try solve [inv hi].
     apply NMF.find_mapsto_iff in hf.
     apply NMF.elements_mapsto_iff in hf.
@@ -700,6 +702,7 @@ Module DefsFn (Export Ty : SYMBOL_TYPES).
     exists (x', yss'); split; auto.
   Qed.
 
+(*
   Lemma in_grammar__keySet :
     forall g pm x ys,
       production_map_correct pm g
@@ -713,9 +716,12 @@ Module DefsFn (Export Ty : SYMBOL_TYPES).
   
   Definition rhsLengths (g : grammar) : list nat :=
     map (fun rhs => List.length rhs) (rhss g).
-
+ *)
+  
   (* The next two definitions help us use a well-founded measure that is 
      already defined in terms of a grammar, rather than a production map *)
+
+  (*
   Definition decompress (e : nonterminal * list (list symbol)) : list production :=
     match e with
     | (x, yss) => map (pair x) yss
@@ -756,7 +762,7 @@ Module DefsFn (Export Ty : SYMBOL_TYPES).
            (prs : list (nonterminal * list (list symbol))),
       In (x, yss) prs
       -> In x (fold_right (fun pr l => fst pr :: l) [] prs).
-    intros x yss prs hi; induction prs as [| (x', yss') prs IH]; sis; auto.
+    intros x yss prs hi; induction prs as [| (x', yss') prs Ih]; sis; auto.
     destruct hi as [hh | ht]; auto.
     inv hh; auto.
   Qed.
@@ -789,8 +795,8 @@ Module DefsFn (Export Ty : SYMBOL_TYPES).
       In rhs (rhss g)
       -> In (List.length rhs) (rhsLengths g).
   Proof.
-    intros g rhs Hin; induction g as [| (x, rhs') ps IH];
-      simpl in *; inv Hin; auto.
+    intros g rhs hin; induction g as [| (x, rhs') ps Ih];
+      simpl in *; inv hin; auto.
   Qed.
 
   Definition maxRhsLength (g : grammar) : nat :=
@@ -813,8 +819,8 @@ Module DefsFn (Export Ty : SYMBOL_TYPES).
       In (x, rhs) g
       -> List.length rhs < 1 + maxRhsLength g.
   Proof.
-    intros g x rhs Hin.
-    apply grammar_rhs_length_le_max in Hin; omega.
+    intros g x rhs hin.
+    apply grammar_rhs_length_le_max in hin; omega.
   Qed.
 
   Definition allNts (g : grammar) : NtSet.t := 
@@ -838,19 +844,18 @@ Module DefsFn (Export Ty : SYMBOL_TYPES).
     apply allNts_lhss_iff. 
     eapply production_lhs_in_lhss; eauto.
   Qed.
-
+   *)
+  
   (* Definitions related to input that the parser consumes. *)
-  Definition literal := string.
-
-  Definition token   := (terminal * literal)% type.
+  Definition token   := {a : terminal & t_semty a}. 
 
   Definition showToken (t : token) : string :=
     match t with
-    | (a, l) => "(" ++ showT a ++ ", " ++ l ++ ")"
+    | @existT _ _ a _ => "(" ++ showT a ++ ")"
     end.
 
-  (* Parser return values *)
-  Inductive tree    := Leaf : terminal -> literal -> tree
+  (* Concrete syntax trees *)
+  Inductive tree    := Leaf : terminal -> tree
                      | Node : nonterminal -> list tree -> tree.
 
   Definition forest := list tree.
@@ -859,7 +864,7 @@ Module DefsFn (Export Ty : SYMBOL_TYPES).
      the output of extracted parsers *)
   Fixpoint countNodes (t : tree) : nat :=
     match t with
-    | Leaf _ _   => 1
+    | Leaf _     => 1
     | Node _ sts =>
       let fix countNodes' (f : forest) : nat :=
           match f with
@@ -869,19 +874,24 @@ Module DefsFn (Export Ty : SYMBOL_TYPES).
       in  countNodes' sts
     end.
 
-  Fixpoint flatten (t : tree) : list token :=
+  Fixpoint flatten (t : tree) : list terminal :=
     match t with
-    | Leaf t l   => [(t,l)]
+    | Leaf t     => [t]
     | Node _ sts => flat_map flatten sts
     end.
 
   (* Parser stacks *)
-  Inductive prefix_frame :=
-  | PF : list symbol -> forest -> prefix_frame.
 
-  Definition prefix_stack := (prefix_frame * list prefix_frame)%type.
+  Inductive frame : Type :=
+  | Fr (x   : nonterminal)       (* lhs *)
+       (pre : list symbol)       (* rhs prefix *)
+       (sem : symbols_semty pre) (* sem value for prefix *)
+       (suf : list symbol).      (* rhs suffix *)
 
-  Inductive suffix_frame :=
+  Definition parser_stack : Type :=
+    (frame * list frame)%type.
+
+(*  Inductive suffix_frame :=
   | SF : option nonterminal -> list symbol -> suffix_frame.
 
   Module SF_as_UOT <: UsualOrderedType.
@@ -953,172 +963,175 @@ Module DefsFn (Export Ty : SYMBOL_TYPES).
   Module TC  := TransClos.Make FS FM.
   
   Definition suffix_stack := (suffix_frame * list suffix_frame)%type. 
+ *)
 
-  Fixpoint unprocTailSyms (frs : list suffix_frame) : list symbol :=
+  Fixpoint unprocSyms (frs : list frame) : list symbol :=
     match frs with 
     | []                         => []
-    | SF _ [] :: _               => [] (* impossible for a well-formed stack *)
-    | SF _ (T _ :: _) :: _       => [] (* impossible for a well-formed stack *)
-    | SF _ (NT x :: suf) :: frs' => suf ++ unprocTailSyms frs'
+    | Fr _ _ _ suf :: frs'       => suf ++ unprocSyms frs'
     end.
 
-  Definition unprocStackSyms (stk : suffix_stack) : list symbol :=
+  Definition unprocStackSyms (stk : parser_stack) : list symbol :=
     match stk with
-    | (SF _ suf, frs) => suf ++ unprocTailSyms frs
+    | (fr, frs) => unprocSyms (fr :: frs)
     end.
 
-  Definition bottomFrameSyms p_stk s_stk := 
-    match bottomElt p_stk, bottomElt s_stk with
-    | PF pre _, SF _ suf => rev pre ++ suf
+  Definition bottomFrameSyms (stk : parser_stack) : list symbol := 
+    match bottomElt stk with
+    | Fr _ pre _ suf => rev pre ++ suf
     end.
 
-  (* Grammatical derivation relation *)
-  Inductive sym_derivation (g : grammar) : symbol -> list token -> tree -> Prop :=
+  (* Grammatical derivation relations -- the main parser correctnes spec *)
+
+  (* Derivation relation for concrete syntax trees *)
+  Inductive tree_derivation (g : grammar) : symbol -> list token -> tree -> Prop :=
   | T_der  : 
-      forall (a : terminal) (l : literal),
-        sym_derivation g (T a) [(a, l)] (Leaf a l)
+      forall (a : terminal) (v : t_semty a),
+        tree_derivation g (T a) [@existT _ _ a v] (Leaf a)
   | NT_der : 
       forall (x  : nonterminal) (ys : list symbol) (w : list token) (sts : forest),
-        In (x, ys) g
-        -> gamma_derivation g ys w sts
-        -> sym_derivation g (NT x) w (Node x sts)
-  with gamma_derivation (g : grammar) : list symbol -> list token-> forest-> Prop :=
+        PM.In (x, ys) g
+        -> forest_derivation g ys w sts
+        -> tree_derivation g (NT x) w (Node x sts)
+  with forest_derivation (g : grammar) : list symbol -> list token-> forest-> Prop :=
        | Nil_der  : 
-           gamma_derivation g [] [] []
+           forest_derivation g [] [] []
        | Cons_der : 
            forall (s : symbol) (ss : list symbol) (wpre wsuf : list token) 
                   (tr : tree) (trs : list tree),
-             sym_derivation g s wpre tr
-             -> gamma_derivation g ss wsuf trs
-             -> gamma_derivation g (s :: ss) (wpre ++ wsuf) (tr :: trs).
+             tree_derivation g s wpre tr
+             -> forest_derivation g ss wsuf trs
+             -> forest_derivation g (s :: ss) (wpre ++ wsuf) (tr :: trs).
 
-  Hint Constructors sym_derivation gamma_derivation : core.
+  Hint Constructors tree_derivation forest_derivation : core.
 
-  Scheme sym_derivation_mutual_ind   := Induction for sym_derivation Sort Prop
-    with gamma_derivation_mutual_ind := Induction for gamma_derivation Sort Prop.
+  Scheme tree_derivation_mutual_ind   := Induction for tree_derivation Sort Prop
+    with forest_derivation_mutual_ind := Induction for forest_derivation Sort Prop.
 
-  Ltac inv_sd hs  hi hg:=
+  Ltac inv_td hs  hi hg:=
     inversion hs as [ ? ? | ? ? ? ? hi hg]; subst; clear hs.
 
-  Ltac inv_gd hg  hs hg' :=
+  Ltac inv_fd hg  hs hg' :=
     inversion hg as [| ? ? ? ? ? ? hs hg']; subst; clear hg.
 
-  Lemma gamma_derivation_app' :
+  Lemma forest_derivation_app' :
     forall g ys1 w1 v1,
-      gamma_derivation g ys1 w1 v1
+      forest_derivation g ys1 w1 v1
       -> forall ys2 w2 v2,
-        gamma_derivation g ys2 w2 v2
-        -> gamma_derivation g (ys1 ++ ys2) (w1 ++ w2) (v1 ++ v2).
+        forest_derivation g ys2 w2 v2
+        -> forest_derivation g (ys1 ++ ys2) (w1 ++ w2) (v1 ++ v2).
   Proof.
     intros g ys1 w1 v1 hg.
     induction hg; intros ys2 w2 v2 hg2; simpl in *; auto.
     rewrite <- app_assoc; constructor; auto.
   Qed.
 
-  Lemma gamma_derivation_app :
+  Lemma forest_derivation_app :
     forall g ys ys' w w' v v',
-      gamma_derivation g ys w v
-      -> gamma_derivation g ys' w' v'
-      -> gamma_derivation g (ys ++ ys') (w ++ w') (v ++ v').
+      forest_derivation g ys w v
+      -> forest_derivation g ys' w' v'
+      -> forest_derivation g (ys ++ ys') (w ++ w') (v ++ v').
   Proof.
-    intros; eapply gamma_derivation_app'; eauto.
+    intros; eapply forest_derivation_app'; eauto.
   Qed.
 
   Lemma forest_app_singleton_node : 
     forall g x ys ys' w w' v v',
-      In (x, ys') g
-      -> gamma_derivation g ys w v
-      -> gamma_derivation g ys' w' v'
-      -> gamma_derivation g (ys ++ [NT x]) (w ++ w') (v ++ [Node x v']).
+      PM.In (x, ys') g
+      -> forest_derivation g ys w v
+      -> forest_derivation g ys' w' v'
+      -> forest_derivation g (ys ++ [NT x]) (w ++ w') (v ++ [Node x v']).
   Proof.
     intros g x ys ys' w w' v v' hi hg hg'.
-    apply gamma_derivation_app; auto.
+    apply forest_derivation_app; auto.
     rew_nil_r w'; eauto.
   Qed.
 
-  Lemma terminal_head_gamma_derivation :
-    forall g a l ys w v,
-      gamma_derivation g ys w v
-      -> gamma_derivation g (T a :: ys) ((a, l) :: w) (Leaf a l :: v).
+  Lemma terminal_head_forest_derivation :
+    forall g a v ys w ts,
+      forest_derivation g ys w ts
+      -> forest_derivation g (T a :: ys) ((@existT _ _ a v) :: w) (Leaf a :: ts).
   Proof.
-    intros g a l ys w v hg.
-    assert (happ : (a, l) :: w = [(a, l)] ++ w) by apply cons_app_singleton.
+    intros g a v ys w ts hg.
+    assert (happ : (@existT _ _  a v) :: w =
+                   [@existT _ _ a v] ++ w)
+      by apply cons_app_singleton.
     rewrite happ; auto.
   Qed.
 
-  Lemma gamma_derivation_split :
+  Lemma forest_derivation_split :
     forall g ys ys' w'' v'',
-      gamma_derivation g (ys ++ ys') w'' v''
+      forest_derivation g (ys ++ ys') w'' v''
       -> exists w w' v v',
         w'' = w ++ w'
         /\ v'' = v ++ v'
-        /\ gamma_derivation g ys  w  v
-        /\ gamma_derivation g ys' w' v'.
+        /\ forest_derivation g ys  w  v
+        /\ forest_derivation g ys' w' v'.
   Proof.
-    intros g ys; induction ys as [| y ys IH]; intros ys' w'' v'' hg; sis.
+    intros g ys; induction ys as [| y ys Ih]; intros ys' w'' v'' hg; sis.
     - exists []; exists w''; exists []; exists v''; repeat split; auto.
     - inversion hg as [| s ss wpre wsuf t f hs hg']; subst; clear hg. 
-      apply IH in hg'; destruct hg' as [w [w' [v [v' [? [? [hg' hg'']]]]]]]; subst.
+      apply Ih in hg'; destruct hg' as [w [w' [v [v' [? [? [hg' hg'']]]]]]]; subst.
       exists (wpre ++ w); exists w'; exists (t :: v); exists v'. 
       repeat split; auto; apps.
   Qed.
 
-  Lemma gamma_derivation_terminal_end :
+  Lemma forest_derivation_terminal_end :
     forall g ys a w v,
-      gamma_derivation g (ys ++ [T a]) w v
+      forest_derivation g (ys ++ [T a]) w v
       -> exists w_front l v_front,
-        w = w_front ++ [(a, l)]
-        /\ v = v_front ++ [Leaf a l]
-        /\ gamma_derivation g ys w_front v_front.
+        w = w_front ++ [@existT _ _ a l]
+        /\ v = v_front ++ [Leaf a]
+        /\ forest_derivation g ys w_front v_front.
   Proof.
     intros g ys a w v hg.
-    eapply gamma_derivation_split in hg.
+    eapply forest_derivation_split in hg.
     destruct hg as [w' [w'' [v' [v'' [? [? [hg hg']]]]]]]; subst.
-    inv hg'.
-    (* lemma *)
-    inv H1. inv H4.
+    inv_fd hg' ht hg''.
+    inv_td ht hi hf.
+    inv_fd hg'' ht hg'''.
     repeat eexists; eauto.
   Qed.
 
-  Lemma gamma_derivation_nonterminal_end :
+  Lemma forest_derivation_nonterminal_end :
     forall g ys x w v,
-      gamma_derivation g (ys ++ [NT x]) w v
+      forest_derivation g (ys ++ [NT x]) w v
       -> exists wpre wsuf vpre v',
         w = wpre ++ wsuf
         /\ v = vpre ++ [Node x v']
-        /\ gamma_derivation g ys wpre vpre
-        /\ sym_derivation g (NT x) wsuf (Node x v').
+        /\ forest_derivation g ys wpre vpre
+        /\ tree_derivation g (NT x) wsuf (Node x v').
   Proof.
     intros g ys x w v hg.
-    eapply gamma_derivation_split in hg.
+    eapply forest_derivation_split in hg.
     destruct hg as [w' [w'' [v' [v'' [? [? [hg hg']]]]]]]; subst.
-    inv hg'.
-    (* lemma *)
-    inv H4. rewrite app_nil_r in *.
-    inv H1.
+    inv_fd hg' ht hg''.
+    inv_td ht hi hf.
+    inv_fd hg'' ht hg'''.
+    rewrite app_nil_r.
     repeat eexists; eauto.
   Qed.
 
-  Lemma trees_eq__gammas_eq_words_eq' :
+(*  Lemma trees_eq__forests_eq_words_eq' :
     forall g ys w v,
-      gamma_derivation g ys w v
+      forest_derivation g ys w v
       -> forall ys' w',
-        gamma_derivation g ys' w' v
+        forest_derivation g ys' w' v
         -> ys' = ys /\ w' = w.
   Proof.
     intros g ys w v hg.
-    induction hg using gamma_derivation_mutual_ind with
-        (P := fun s w t (hs : sym_derivation g s w t) =>
+    induction hg using forest_derivation_mutual_ind with
+        (P := fun s w t (hs : tree_derivation g s w t) =>
                 forall s' w',
-                  sym_derivation g s' w' t
+                  tree_derivation g s' w' t
                   -> s' = s /\ w' = w).
     - intros s' w' hs; inv hs; auto.
     - intros s' w' hs; inv hs; firstorder.
     - intros ys' w' hg; inv hg; auto.
     - intros ys' w' hg'; inv hg'.
-      apply IHhg in H3; destruct H3; subst.
-      apply IHhg0 in H4; destruct H4; subst; auto.
-  Qed.
+      apply Ihhg in h3; destruct h3; subst.
+      apply Ihhg0 in h4; destruct h4; subst; auto.
+  Qed. 
 
   Lemma trees_eq__gammas_eq_words_eq :
     forall g ys ys' w w' v,
@@ -1129,42 +1142,44 @@ Module DefsFn (Export Ty : SYMBOL_TYPES).
     intros; eapply trees_eq__gammas_eq_words_eq'; eauto.
   Qed.
 
-  Lemma gamma_derivation_singleton_t :
+ *)
+
+  Lemma forest_derivation_singleton_t :
     forall g a w v,
-      gamma_derivation g [T a] w v
+      forest_derivation g [T a] w v
       -> exists l,
-        w = [(a, l)]
-        /\ v = [Leaf a l].
+        w = [@existT _ _ a l]
+        /\ v = [Leaf a].
   Proof.
     intros g a w v hg.
-    inv_gd hg hs hg'.
+    inv_fd hg hs hg'.
     inv hs; inv hg'; rewrite app_nil_r; eauto.
   Qed.
 
-  Lemma gamma_derivation_singleton_nt :
+  Lemma forest_derivation_singleton_nt :
     forall g x w v,
-      gamma_derivation g [NT x] w v
+      forest_derivation g [NT x] w v
       -> exists ys v',
-        In (x, ys) g
+        PM.In (x, ys) g
         /\ v = [Node x v']
-        /\ gamma_derivation g ys w v'.
+        /\ forest_derivation g ys w v'.
   Proof.
     intros g x w v hg.
-    inv_gd hg hs hg'.
+    inv_fd hg hs hg'.
     inv hs; inv hg'; rewrite app_nil_r; eauto.
   Qed.
 
-  Definition unique_gamma_derivation g ss w v :=
-    gamma_derivation g ss w v
-    /\ forall v', gamma_derivation g ss w v' -> v = v'.
+  Definition unique_forest_derivation g ss w v :=
+    forest_derivation g ss w v
+    /\ forall v', forest_derivation g ss w v' -> v = v'.
 
   Inductive sym_recognize (g : grammar) : symbol -> list token -> Prop :=
   | T_rec  : 
-      forall (a : terminal) (l : literal),
-        sym_recognize g (T a) [(a, l)]
+      forall (a : terminal) (l : t_semty a),
+        sym_recognize g (T a) [@existT _ _ a l]
   | NT_rec : 
       forall (x  : nonterminal) (ys : list symbol) (w : list token),
-        In (x, ys) g
+        PM.In (x, ys) g
         -> gamma_recognize g ys w
         -> sym_recognize g (NT x) w
   with gamma_recognize (g : grammar) : list symbol -> list token -> Prop :=
@@ -1187,14 +1202,14 @@ Module DefsFn (Export Ty : SYMBOL_TYPES).
   Scheme sym_recognize_mutual_ind   := Induction for sym_recognize Sort Prop
     with gamma_recognize_mutual_ind := Induction for gamma_recognize Sort Prop.
 
-  Lemma sym_derivation__sym_recognize :
+  Lemma tree_derivation__sym_recognize :
     forall g s w v,
-      sym_derivation g s w v
+      tree_derivation g s w v
       -> sym_recognize g s w.
   Proof.
     intros g ys w v hs.
-    induction hs using sym_derivation_mutual_ind
-      with (P0 := fun ys w f (hg : gamma_derivation g ys w f) => 
+    induction hs using tree_derivation_mutual_ind
+      with (P0 := fun ys w f (hg : forest_derivation g ys w f) => 
                     gamma_recognize g ys w); eauto.
   Qed.
 
@@ -1202,7 +1217,7 @@ Module DefsFn (Export Ty : SYMBOL_TYPES).
     forall g a suf w,
       gamma_recognize g (T a :: suf) w
       -> exists l w',
-        w = (a, l) :: w'
+        w = (@existT _ _ a l) :: w'
         /\ gamma_recognize g suf w'.
   Proof.
     intros g a suf w hg.
@@ -1215,7 +1230,7 @@ Module DefsFn (Export Ty : SYMBOL_TYPES).
       gamma_recognize g (NT x :: suf) w
       -> exists rhs wpre wsuf,
         w = wpre ++ wsuf
-        /\ In (x, rhs) g
+        /\ PM.In (x, rhs) g
         /\ gamma_recognize g rhs wpre
         /\ gamma_recognize g suf wsuf.
   Proof.
@@ -1253,16 +1268,16 @@ Module DefsFn (Export Ty : SYMBOL_TYPES).
         /\ gamma_recognize g ys w
         /\ gamma_recognize g ys' w'.
   Proof.
-    intros g ys; induction ys as [| y ys IH]; intros ys' w'' hg; sis.
+    intros g ys; induction ys as [| y ys Ih]; intros ys' w'' hg; sis.
     - exists []; exists w''; repeat split; auto.
     - inversion hg as [| s ss wpre wsuf hs hg']; subst; clear hg. 
-      apply IH in hg'; destruct hg' as [w [w' [? [hg' hg'']]]]; subst.
+      apply Ih in hg'; destruct hg' as [w [w' [? [hg' hg'']]]]; subst.
       exists (wpre ++ w); exists w'; repeat split; auto; apps.
   Qed.
 
   Lemma gamma_recognize_fold_head_nt :
     forall g x rhs ys ts,
-      In (x, rhs) g
+      PM.In (x, rhs) g
       -> gamma_recognize g (rhs ++ ys) ts
       -> gamma_recognize g (NT x :: ys) ts.
   Proof.
@@ -1271,34 +1286,34 @@ Module DefsFn (Export Ty : SYMBOL_TYPES).
     destruct hr as [w [w' [? [hr hr']]]]; subst; eauto.
   Qed.
 
-  Lemma gamma_derivation__gamma_recognize :
+  Lemma forest_derivation__gamma_recognize :
     forall g ys w v,
-      gamma_derivation g ys w v
+      forest_derivation g ys w v
       -> gamma_recognize g ys w.
   Proof.
     intros g ys w v hg.
-    induction hg using gamma_derivation_mutual_ind with
-        (P := fun s w t (hs : sym_derivation g s w t) => 
+    induction hg using forest_derivation_mutual_ind with
+        (P := fun s w t (hs : tree_derivation g s w t) => 
                 sym_recognize g s w); eauto.
   Qed.
 
-  Lemma gamma_recognize__exists_gamma_derivation :
+  Lemma gamma_recognize__exists_forest_derivation :
     forall g ys w,
       gamma_recognize g ys w
       -> exists v,
-        gamma_derivation g ys w v.
+        forest_derivation g ys w v.
   Proof.
     intros g ys w hg.
     induction hg using gamma_recognize_mutual_ind with
         (P := fun s w (hs : sym_recognize g s w) => 
-                exists t, sym_derivation g s w t); firstorder; eauto.
-    repeat econstructor; eauto.
+                exists t, tree_derivation g s w t);
+      firstorder; repeat econstructor; eauto.
   Qed.
 
   (* Inductive definition of a nullable grammar symbol *)
   Inductive nullable_sym (g : grammar) : symbol -> Prop :=
   | NullableSym : forall x ys,
-      In (x, ys) g
+      PM.In (x, ys) g
       -> nullable_gamma g ys
       -> nullable_sym g (NT x)
   with nullable_gamma (g : grammar) : list symbol -> Prop :=
@@ -1315,7 +1330,7 @@ Module DefsFn (Export Ty : SYMBOL_TYPES).
       nullable_gamma g (xs ++ ys)
       -> nullable_gamma g xs /\ nullable_gamma g ys.
   Proof.
-    intros g xs; induction xs as [| x xs IH]; intros ys hn; sis; auto.
+    intros g xs; induction xs as [| x xs Ih]; intros ys hn; sis; auto.
     inv hn; firstorder.
   Qed.
 
@@ -1340,12 +1355,12 @@ Module DefsFn (Export Ty : SYMBOL_TYPES).
   Inductive nullable_path (g : grammar) :
     symbol -> symbol -> Prop :=
   | DirectPath : forall x z gamma pre suf,
-      In (x, gamma) g
+      PM.In (x, gamma) g
       -> gamma = pre ++ NT z :: suf
       -> nullable_gamma g pre
       -> nullable_path g (NT x) (NT z)
   | IndirectPath : forall x y z gamma pre suf,
-      In (x, gamma) g
+      PM.In (x, gamma) g
       -> gamma = pre ++ NT y :: suf
       -> nullable_gamma g pre
       -> nullable_path g (NT y) (NT z)
